Freigen/CompM/Basic.lean
@@ -1,0 +1,62 @@
+import Freigen.ITree.Basic
+import Freigen.CompM.ExactCodensity
+
+namespace Freigen
+
+def CompM (E : ITree.EffSpec) (α : Type) : Type _ := CompM.ExactCodensity (ITree E) α
+
+instance {E} : Monad (CompM E) := inferInstanceAs (Monad (CompM.ExactCodensity (ITree E)))
+instance {E} : LawfulMonad (CompM E) := inferInstanceAs (LawfulMonad (CompM.ExactCodensity (ITree E)))
+
+namespace CompM
+
+variable { E : ITree.EffSpec } { α β : Type }
+
+private theorem bind_def {α β : Type _} (x : CompM E α) (f : α → CompM E β) :
+    x >>= f = ⟨fun g => x.run fun a => (f a).run g, by
+      intros
+      conv => lhs; rw [←x.exact]
+      rw [bind_assoc]
+      simp only [ExactCodensity.exact]⟩ := by
+  rfl
+
+def tick : CompM E Unit := ⟨fun f => ITree.tau (f ()), by simp⟩
+def op (e : E.tag) (inp : E.input e)
+    (blocks : (t : E.blockTag e) → E.blockInputs e t → ITree E (E.blockOutputs e t)): CompM E (E.output e) :=
+  ⟨fun f => ITree.op e inp blocks f, by simp⟩
+def fail : CompM E α := ⟨fun _ => ITree.fail, by simp⟩
+
+@[simp]
+theorem fail_bind (f : α → CompM E β) : fail >>= f = fail := by
+  simp [fail, bind_def]
+
+def loop (body : α → CompM E (ForInStep α)) (init : α): CompM E α := {
+  run := fun f => ITree.loop (fun a => (body a).run pure) init f
+  exact := by
+    intros
+    apply ITree.loop_bind
+}
+
+theorem loop_def
+  (body : β → CompM E (ForInStep β))
+  (s : β) :
+  CompM.loop body s =
+    body s >>= fun
+      | .done v  => pure v
+      | .yield v => CompM.tick *> CompM.loop body v := by
+  apply (ExactCodensity.equiv β).injective
+  change (CompM.loop body s).run pure =
+    ((body s >>= fun
+      | .done v => pure v
+      | .yield v => CompM.tick *> CompM.loop body v) : CompM E β).run pure
+  simp only [loop, bind_def]
+  rw [ITree.loop_def]
+  rw [ExactCodensity.exact]
+  congr 1
+  funext x
+  cases x <;> rfl
+
+instance : ForIn (CompM E) Lean.Loop Unit where
+  forIn _ init body := loop (fun a => body () a) init
+
+end Freigen.CompM
