Freigen/CompM/ExactCodensity.lean
@@ -1,0 +1,39 @@
+import Mathlib.Logic.Equiv.Defs
+
+namespace Freigen.CompM
+
+structure ExactCodensity (M : Type u → Type v) [Monad M] (α : Type _) where
+  run : ∀ {β : Type u}, (α → M β) → M β
+  exact : ∀ {β : Type u} (f : α → M β), run pure >>= f = run f
+
+instance {M} [Monad M] [LawfulMonad M] : Monad (ExactCodensity M) where
+  pure a := ⟨fun f => f a, by simp⟩
+  bind x f := {
+    run := fun g => x.run fun a => (f a).run g,
+    exact := by
+      intros
+      conv => lhs; rw [←x.exact]
+      rw [bind_assoc]
+      simp only [ExactCodensity.exact]
+  }
+
+instance {M} [Monad M] [LawfulMonad M] : LawfulMonad (ExactCodensity M) := LawfulMonad.mk' _
+  (by intros; rfl)
+  (by intros; rfl)
+  (by intros; rfl)
+
+protected def ExactCodensity.equiv {M} [Monad M] [LawfulMonad M] (α : Type u) : ExactCodensity M α ≃ M α where
+  toFun x := x.run pure
+  invFun x := ⟨fun f => x >>= f, by simp⟩
+  left_inv x := by simp only [ExactCodensity.exact]
+  right_inv x := by simp
+
+def ExactCodensity.bind_def {M} [Monad M] [LawfulMonad M] {α β : Type _} (x : ExactCodensity M α) (f : α → ExactCodensity M β) :
+    x >>= f = ⟨fun g => x.run fun a => (f a).run g, by
+      intros
+      conv => lhs; rw [←x.exact]
+      rw [bind_assoc]
+      simp only [ExactCodensity.exact]⟩ := by
+  rfl
+
+end Freigen.CompM
